theories/sts.v
@@ -3,66 +3,78 @@ From iris.base_logic Require Export invariants.
 From iris.proofmode Require Import tactics.
 Import uPred.
 
-
 (** The CMRA for the heap of STS.
-    We register the state and the transition relation. *)
-Definition sts_stateUR := authUR (gmapUR positive (exclR (leibnizO positive))).
+    We distinguish between the standard and owned sts. *) 
 
+(** For shared resources, we register the state. *)
+
+Definition sts_std_stateUR (A B : Type) {eqD: EqDecision A} {count: Countable A} := authUR (gmapUR A (exclR (leibnizO B))).
+Definition STS_std_states (A B : Type) {eqD: EqDecision A} {count: Countable A} : Type := gmap A B.
+
+
+(** For owned resources, we register the state and the transition relation. *)
+
+Definition sts_stateUR := authUR (gmapUR positive (exclR (leibnizO positive))).
 Definition sts_relUR :=
   authUR (gmapUR positive (agreeR (leibnizO ((positive → positive → Prop) * (positive → positive → Prop))))).
 
 Definition STS_states : Type := gmap positive positive.
 Definition STS_rels : Type := gmap positive ((positive → positive → Prop) * (positive → positive → Prop)).
 
-(** The CMRA for the thread pool. *)
-Class STSG Σ :=
-  { sts_state_inG :> inG Σ sts_stateUR;
+(** Standard STS. *)
+Class STS_STD (B : Type) :=
+  { Rpub : relation B;
+    Rpriv : relation B;}.
+
+(** The CMRA for the sts collection. *)
+Class STSG A B Σ {eqd: EqDecision A} {count: Countable A} :=
+  { (* eqDA :> EqDecision A;  *)
+    (* countA :> Countable A; *)
+    sts_state_inG :> inG Σ sts_stateUR;
+    sts_std_state_inG :> inG Σ (sts_std_stateUR A B);
     sts_rel_inG :> inG Σ sts_relUR;
     γs_std : gname;
     γs_loc : gname;
     γr_std : gname;
     γr_loc : gname;}.
 
-Class STS_STD A :=
-  { Rpub : relation A;
-    Rpriv : relation A;}. 
-
 Section definitionsS.
-  Context `{STSG Σ} `{Countable A} `{Countable B}.
+  Context {A B C D: Type} {Σ : gFunctors} {eqa: EqDecision A} {count: Countable A}
+          {sts_std: STS_STD B} {eqc : EqDecision C} {countC: Countable C}
+          {eqd : EqDecision D} {countD: Countable D} {stsg : STSG A B Σ}.
   Notation STS := (leibnizO (STS_states * STS_rels)).
-  Notation WORLD := (prodO STS STS). 
+  Notation STS_STD := (leibnizO (STS_std_states A B)).
+  Notation WORLD := (prodO STS_STD STS). 
   Implicit Types W : WORLD.
-
-  Definition sts_state_std (i : positive) (x : A) : iProp Σ
-    := own (A := sts_stateUR) γs_std (◯ {[ i := Excl (encode x) ]}).
-
-  Definition sts_state_loc (i : positive) (y : B) : iProp Σ
-    := own (A := sts_stateUR) γs_loc (◯ {[ i := Excl (encode y) ]}).
-
-  Definition convert_rel {A : Type} `{Countable A} (R : A → A → Prop) : positive → positive → Prop :=
-    λ x y, ∃ a b, x = encode a ∧ y = encode b ∧ R a b.
-
-  (* for the standard map we will only have the standard sts *)
-  Definition sts_rel_std (sts_std : STS_STD A) (i : positive) : iProp Σ :=
-    own (A := sts_relUR) γr_std (◯ {[ i := to_agree ((convert_rel (A:=A) Rpub,convert_rel (A:=A) Rpriv)) ]}).
   
-  Definition sts_rel_loc (i : positive) (R : B → B → Prop) (P : B → B → Prop) : iProp Σ :=
-    own (A := sts_relUR) γr_loc (◯ {[ i := to_agree ((convert_rel R,convert_rel P)) ]}).
 
-  Definition sts_subset (fr : STS_rels) : Prop :=
-    ∀ i (r r' : positive → positive → Prop),
-      fr !! i = Some (r,r') → (∀ a b, r a b → r' a b). 
+  Program Definition sts_state_std (i : A) (x : B) : iProp Σ
+    := own (γs_std (A:=A)) (◯ {[ i := Excl x ]}).
 
-  Program Definition sts_full `{STSG Σ} γs γr (fs : STS_states) (fr : STS_rels) : iProp Σ
+  Definition sts_state_loc (i : positive) (y : D) : iProp Σ
+    := own (γs_loc (A:=A)) (◯ {[ i := Excl (encode y) ]}).
+
+  Definition convert_rel {D : Type} `{Countable D} (R : D → D → Prop) : positive → positive → Prop :=
+    λ x y, ∃ a b, x = encode a ∧ y = encode b ∧ R a b.
+  
+  Definition sts_rel_loc (i : positive) (R : D → D → Prop) (P : D → D → Prop) : iProp Σ :=
+    own (γr_loc (A:=A)) (◯ {[ i := to_agree ((convert_rel R,convert_rel P)) ]}).
+
+  Program Definition sts_full γs γr (fs : STS_states) (fr : STS_rels) : iProp Σ
     := (own (A := sts_stateUR) γs (● (Excl <$> fs))
             ∗ own (A := sts_relUR) γr (● (to_agree <$> fr)))%I.
-  Program Definition sts_full_std `{STSG Σ} (sts_std : STS_STD A) γs γr (fs : STS_states) (fr : STS_rels) : iProp Σ
-    := (⌜dom (gset positive) fs ⊆ dom (gset positive) fr⌝
-       ∗ ⌜∀ (i : positive), is_Some(fr !! i) → fr !! i = Some (convert_rel (A:=A) Rpub,convert_rel (A:=A) Rpriv)⌝
-       ∗ own (A := sts_stateUR) γs (● (Excl <$> fs))
-       ∗ own (A := sts_relUR) γr (● (to_agree <$> fr)))%I.
-  Program Definition sts_full_world `{STSG Σ} (sts_std : STS_STD A) W : iProp Σ :=
-    ((sts_full_std sts_std γs_std γr_std W.1.1 W.1.2) ∗ (sts_full γs_loc γr_loc W.2.1 W.2.2))%I. 
+  Program Definition sts_full_std γs (fs : STS_std_states A B) : iProp Σ
+    := own (A := sts_std_stateUR A B) γs (● (Excl <$> fs))%I.
+  Program Definition sts_full_world W : iProp Σ :=
+    ((sts_full_std (γs_std (A:=A)) W.1) ∗ (sts_full (γs_loc (A:=A)) (γr_loc (A:=A)) W.2.1 W.2.2))%I.
+
+  Definition related_sts_std_pub (fs gs : STS_std_states A B) : Prop :=
+    dom (gset A) fs ⊆ dom (gset A) gs ∧
+    ∀ i x y, fs !! i = Some x → gs !! i = Some y → rtc (Rpub) x y.
+
+  Definition related_sts_std_priv (fs gs : STS_std_states A B) : Prop :=
+    dom (gset A) fs ⊆ dom (gset A) gs ∧
+    ∀ i x y, fs !! i = Some x → gs !! i = Some y → rtc (λ x y, (Rpub x y ∨ Rpriv x y)) x y.
 
   Definition related_sts_pub (fs gs : STS_states) (fr gr : STS_rels) : Prop :=
     dom (gset positive) fs ⊆ dom (gset positive) gs ∧
@@ -79,20 +91,16 @@ Section definitionsS.
                        (∀ x y, fs !! i = Some x → gs !! i = Some y → (rtc (λ x y, (r1 x y ∨ r2 x y)) x y)).
 
   Definition related_sts_pub_world W W' :=
-    related_sts_pub W.1.1 W'.1.1 W.1.2 W'.1.2 ∧
+    related_sts_std_pub W.1 W'.1 ∧
     related_sts_pub W.2.1 W'.2.1 W.2.2 W'.2.2.
 
   Definition related_sts_priv_world W W' :=
-    related_sts_priv W.1.1 W'.1.1 W.1.2 W'.1.2 ∧
+    related_sts_std_priv W.1 W'.1 ∧
     related_sts_priv W.2.1 W'.2.1 W.2.2 W'.2.2.
 
-  Global Instance sts_rel_std_Persistent i sts_stg : Persistent (sts_rel_std sts_stg i).
-  Proof. apply _. Qed.
   Global Instance sts_rel_loc_Persistent i R P : Persistent (sts_rel_loc i R P).
   Proof. apply _. Qed.
   
-  Global Instance sts_rel_std_Timeless i sts_stg : Timeless (sts_rel_std sts_stg i).
-  Proof. apply _. Qed.
   Global Instance sts_rel_loc_Timeless i R P : Timeless (sts_rel_loc i R P).
   Proof. apply _. Qed.
   
@@ -103,12 +111,12 @@ Section definitionsS.
   
   Global Instance sts_full_Timeless γs γr fs fr : Timeless (sts_full γs γr fs fr).
   Proof. apply _. Qed.
-  Global Instance sts_full_world_Timeless sts_stg W : Timeless (sts_full_world sts_stg W). 
+  Global Instance sts_full_world_Timeless W : Timeless (sts_full_world W). 
   Proof. apply _. Qed. 
   
 End definitionsS.
 
-Typeclasses Opaque sts_state_std sts_state_loc sts_rel_std sts_rel_loc sts_full
+Typeclasses Opaque sts_state_std sts_state_loc sts_rel_loc sts_full
             related_sts_pub related_sts_priv.
 
 Lemma rtc_implies {A : Type} (R Q : A → A → Prop) (x y : A) :
@@ -144,15 +152,25 @@ Lemma rtc_or_intro_l {A : Type} (R Q : A → A → Prop) (x y : A) :
   Qed.
     
 Section STS.
-  Context `{STSG Σ} `{Countable A} `{sts_std : STS_STD A} `{Countable B}.
+  Context {A B C D: Type} {Σ : gFunctors} {eqa: EqDecision A} {count: Countable A}
+          {sts_std: STS_STD B} {eqc : EqDecision C} {countC: Countable C}
+          {eqd : EqDecision D} {countD: Countable D} {stsg : STSG A B Σ}.
   Implicit Types x y : positive.
   Implicit Types a : A.
-  Implicit Types b : B. 
+  Implicit Types b : B.
+  Implicit Types c : C.
+  Implicit Types d : D.
   Implicit Types fs gs : STS_states.
+  Implicit Types fsd gsd : STS_std_states A B.
   Implicit Types fr_pub fr_priv gr_pub gr_priv : STS_rels.
-  Implicit Types R : A → A → Prop.
-  Implicit Types Q : B → B → Prop. 
+  Implicit Types R : C → C → Prop.
+  Implicit Types Q : D → D → Prop. 
   Implicit Types Rp : positive → positive → Prop.
+
+  Notation STS := (leibnizO (STS_states * STS_rels)).
+  Notation STS_STD := (leibnizO (STS_std_states A B)).
+  Notation WORLD := (prodO STS_STD STS). 
+  Implicit Types W : WORLD.
 
   Lemma elem_of_gmap_dom {K V : Type} `{EqDecision K} `{Countable K}
         (m : gmap K V) (i : K) :
@@ -182,19 +200,51 @@ Section STS.
     eauto using rtc_refl.
   Qed.
 
+  Lemma related_sts_std_pub_refl fsd : related_sts_std_pub fsd fsd.
+  Proof.
+    split; trivial.
+    intros; simplify_eq.
+    eauto using rtc_refl.
+  Qed.
+
+  Lemma related_sts_std_priv_refl fsd : related_sts_std_priv fsd fsd.
+  Proof.
+    split; trivial.
+    intros; simplify_eq.
+    eauto using rtc_refl.
+  Qed.
+
+  Lemma related_sts_pub_refl_world W : related_sts_pub_world W W.
+  Proof. split;[apply related_sts_std_pub_refl|apply related_sts_pub_refl]. Qed.
+  Lemma related_sts_priv_refl_world W : related_sts_priv_world W W.
+  Proof. split;[apply related_sts_std_priv_refl|apply related_sts_priv_refl]. Qed. 
+  
   Lemma related_sts_pub_priv fs fr gs gr :
     related_sts_pub fs gs fr gr → related_sts_priv fs gs fr gr.
   Proof.
     rewrite /related_sts_pub /related_sts_priv. 
     intros [Hf1 [Hf2 Hf3]].
     do 2 (split; auto). intros. 
-    specialize (Hf3 i r1 r2 r1' r2' H2 H3) as (Hr1 & Hr2 & Hrtc); auto.
+    specialize (Hf3 i r1 r2 r1' r2' H H0) as (Hr1 & Hr2 & Hrtc); auto.
     subst. repeat (split;auto). intros.
-    specialize (Hrtc x y H4 H5). 
+    specialize (Hrtc x y H1 H2). 
     inversion Hrtc.
     - left.
     - right with y0; auto.
-      apply rtc_or_intro. apply H7. 
+      apply rtc_or_intro. apply H4. 
+  Qed.
+
+  Lemma related_sts_std_pub_priv fsd gsd :
+    related_sts_std_pub fsd gsd → related_sts_std_priv fsd gsd.
+  Proof.
+    rewrite /related_sts_pub /related_sts_priv. 
+    intros [Hf1 Hf2].
+    repeat (split; auto). intros. 
+    specialize (Hf2 i _ _ H H0) as Hrtc; auto.
+    inversion Hrtc.
+    - left.
+    - right with y0; auto.
+      apply rtc_or_intro. subst. auto. 
   Qed. 
 
   Lemma related_sts_pub_trans fs fr gs gr hs hr :
@@ -211,6 +261,20 @@ Section STS.
     repeat (split;auto).
     intros x y Hx Hy. 
     destruct Hf1;eauto.
+    etrans;eauto. 
+  Qed.
+
+  Lemma related_sts_std_pub_trans fsd gsd hsd :
+    related_sts_std_pub fsd gsd → related_sts_std_pub gsd hsd →
+    related_sts_std_pub fsd hsd.
+  Proof.
+    intros [Hf1 Hf2] [Hg1 Hg2]; split; try by etrans.
+    intros i x y Hx Hy.
+    specialize (Hf1 i);
+      revert Hf1; rewrite !elem_of_dom; intros Hf1.
+    destruct Hf1 as [x0 Hx0]; eauto.
+    specialize (Hf2 i x x0 Hx Hx0); simplify_eq.
+    specialize (Hg2 i x0 y Hx0 Hy); simplify_eq.
     etrans;eauto. 
   Qed.
   
@@ -232,6 +296,21 @@ Section STS.
     apply rtc_or_intro; auto. 
   Qed.
 
+  Lemma related_sts_std_priv_pub_trans fsd gsd hsd :
+    related_sts_std_priv fsd gsd → related_sts_std_pub gsd hsd →
+    related_sts_std_priv fsd hsd.
+  Proof.
+    intros [Hf1 Hf2] [Hg1 Hg2]; split; try by etrans.
+    intros i x y Hx Hy.
+    specialize (Hf1 i);
+      revert Hf1; rewrite !elem_of_dom; intros Hf1.
+    destruct Hf1 as [x0 Hx0]; eauto.
+    specialize (Hf2 i x x0 Hx Hx0); simplify_eq.
+    specialize (Hg2 i x0 y Hx0 Hy); simplify_eq.
+    etrans;eauto. 
+    apply rtc_or_intro; auto.
+  Qed. 
+
   Lemma related_sts_pub_priv_trans fs fr gs gr hs hr :
     related_sts_pub fs gs fr gr → related_sts_priv gs hs gr hr →
     related_sts_priv fs hs fr hr.
@@ -250,6 +329,21 @@ Section STS.
     apply rtc_or_intro; auto. 
   Qed.
 
+  Lemma related_sts_std_pub_priv_trans fsd gsd hsd :
+    related_sts_std_pub fsd gsd → related_sts_std_priv gsd hsd →
+    related_sts_std_priv fsd hsd.
+  Proof.
+    intros [Hf1 Hf2] [Hg1 Hg2]; split; try by etrans.
+    intros i x y Hx Hy.
+    specialize (Hf1 i);
+      revert Hf1; rewrite !elem_of_dom; intros Hf1.
+    destruct Hf1 as [x0 Hx0]; eauto.
+    specialize (Hf2 i x x0 Hx Hx0); simplify_eq.
+    specialize (Hg2 i x0 y Hx0 Hy); simplify_eq.
+    etrans;eauto. 
+    apply rtc_or_intro; auto.
+  Qed. 
+
   Lemma related_sts_priv_trans fs fr gs gr hs hr :
     related_sts_priv fs gs fr gr → related_sts_priv gs hs gr hr →
     related_sts_priv fs hs fr hr.
@@ -267,6 +361,20 @@ Section STS.
     etrans;eauto. 
   Qed.
 
+  Lemma related_sts_std_priv_trans fsd gsd hsd :
+    related_sts_std_priv fsd gsd → related_sts_std_priv gsd hsd →
+    related_sts_std_priv fsd hsd.
+  Proof.
+    intros [Hf1 Hf2] [Hg1 Hg2]; split; try by etrans.
+    intros i x y Hx Hy.
+    specialize (Hf1 i);
+      revert Hf1; rewrite !elem_of_dom; intros Hf1.
+    destruct Hf1 as [x0 Hx0]; eauto.
+    specialize (Hf2 i x x0 Hx Hx0); simplify_eq.
+    specialize (Hg2 i x0 y Hx0 Hy); simplify_eq.
+    etrans;eauto.
+  Qed.   
+
   (* Helper functions for transitivity of sts pairs *)
   Lemma related_sts_pub_priv_trans_world W W' W'' :
     related_sts_pub_world W W' -> related_sts_priv_world W' W'' ->
@@ -274,7 +382,7 @@ Section STS.
   Proof.
     intros [Hpub_std Hpub_loc] [Hpriv_std Hpriv_loc].
     split. 
-    - apply related_sts_pub_priv_trans with W'.1.1 W'.1.2; auto.
+    - apply related_sts_std_pub_priv_trans with W'.1; auto.
     - apply related_sts_pub_priv_trans with W'.2.1 W'.2.2; auto.
   Qed.
 
@@ -284,7 +392,7 @@ Section STS.
   Proof.
     intros [Hpub_std Hpub_loc] [Hpriv_std Hpriv_loc].
     split. 
-    - apply related_sts_priv_pub_trans with W'.1.1 W'.1.2; auto.
+    - apply related_sts_std_priv_pub_trans with W'.1; auto.
     - apply related_sts_priv_pub_trans with W'.2.1 W'.2.2; auto.
   Qed.
 
@@ -294,7 +402,7 @@ Section STS.
   Proof.
     intros [Hpub_std Hpub_loc] [Hpriv_std Hpriv_loc].
     split. 
-    - apply related_sts_priv_trans with W'.1.1 W'.1.2; auto.
+    - apply related_sts_std_priv_trans with W'.1; auto.
     - apply related_sts_priv_trans with W'.2.1 W'.2.2; auto.
   Qed.
 
@@ -304,7 +412,7 @@ Section STS.
   Proof.
     intros [Hpub_std Hpub_loc] [Hpriv_std Hpriv_loc].
     split. 
-    - apply related_sts_pub_trans with W'.1.1 W'.1.2; auto.
+    - apply related_sts_std_pub_trans with W'.1; auto.
     - apply related_sts_pub_trans with W'.2.1 W'.2.2; auto.
   Qed.
 
@@ -312,61 +420,14 @@ Section STS.
     related_sts_pub_world W W' -> related_sts_priv_world W W'.
   Proof.
     intros [Hstd Hloc].
-    split; apply related_sts_pub_priv; auto.
+    split; [apply related_sts_std_pub_priv|apply related_sts_pub_priv]; auto.
   Qed.
-
-  Lemma sts_full_rel_std W (i : positive) :
-    (sts_full_world sts_std W -∗ sts_rel_std sts_std i -∗
-                    ⌜W.1.2 !! i = Some (convert_rel (Rpub : relation A), convert_rel (Rpriv : relation A))⌝)%I.
-  Proof.
-    rewrite /sts_rel_std /sts_full_world /sts_full.
-    destruct W as [[fs fr] Wloc].
-    (* iIntros "[% [_ H1]] H2". *)
-    iIntros "[[_ [% [_ H1]]] _] H2 /=".
-    iDestruct (own_valid_2 with "H1 H2") as %[HR Hv]%auth_both_valid;
-      iPureIntro.
-    specialize (Hv i).
-    revert HR. rewrite /= singleton_included;
-      intros [z [Hz HR]]; revert HR; rewrite Some_included_total; intros HR.
-    rewrite lookup_fmap in Hz, Hv.
-    destruct (fr !! i) eqn:Heq; rewrite Heq /= in Hz, Hv; last by inversion Hz.
-    revert Hv; rewrite Hz; intros [u Hu]%to_agree_uninj.
-    revert HR; rewrite -Hu; intros HR%to_agree_included%leibniz_equiv;
-      simplify_eq.
-    inversion Hz as [? ? Hz'|]; simplify_eq.
-    revert Hz'; rewrite -Hu. intros Hz'%(to_agree_inj (A:=leibnizO _) p _)%leibniz_equiv. 
-    by rewrite Hz'.  
-  Qed.
-
-  Lemma sts_full_rel_state_std W i a :
-    (sts_full_world sts_std W -∗ sts_state_std i a -∗
-                    ⌜W.1.2 !! i = Some (convert_rel (Rpub : relation A), convert_rel (Rpriv : relation A))⌝)%I.
-  Proof.
-    rewrite /sts_full_world /sts_full /sts_state_std.
-    (* iIntros "[% [H1 _]] H2". *)
-    destruct W as [[fs fr] Wloc]. 
-    iIntros "[[Hdom [Hstd [H1 _] ] ] _] H2".
-    iDestruct "Hdom" as %Hdom. iDestruct "Hstd" as %Hstd.  
-    iDestruct (own_valid_2 with "H1 H2") as %[HR Hv]%auth_both_valid;
-      iPureIntro.
-    specialize (Hv i).
-    revert HR; rewrite /= singleton_included;
-      intros [z [Hz HR]].
-    rewrite lookup_fmap in Hz Hv.
-    destruct (fs !! i) eqn:Heq; rewrite Heq /= in Hz Hv; last by inversion Hz.
-    apply leibniz_equiv in Hz; simplify_eq.
-    revert Hdom. rewrite /= elem_of_subseteq =>Hdom.
-    assert (i ∈ dom (gset positive) fs) as Hin; [apply elem_of_dom;eauto|].
-    specialize (Hdom i Hin). apply elem_of_dom in Hdom.
-    specialize (Hstd i Hdom). done. 
-  Qed. 
     
   Lemma sts_full_rel_loc W i Q P :
-    sts_full_world sts_std W -∗ sts_rel_loc i Q P -∗ ⌜W.2.2 !! i = Some (convert_rel Q,convert_rel P)⌝.
+    sts_full_world W -∗ sts_rel_loc (A:=A) i Q P -∗ ⌜W.2.2 !! i = Some (convert_rel Q,convert_rel P)⌝.
   Proof.
     rewrite /sts_rel_loc /sts_full_world /sts_full.
     destruct W as [Wstd [fs fr]].
-    (* iIntros "[% [_ H1]] H2". *)
     iIntros "[_ [_ H1]] H2 /=".
     iDestruct (own_valid_2 with "H1 H2") as %[HR Hv]%auth_both_valid;
       iPureIntro.
@@ -383,30 +444,28 @@ Section STS.
     by rewrite Hz'.  
   Qed.
       
-  Lemma sts_full_state_std W i a :
-    sts_full_world sts_std W -∗ sts_state_std i a -∗ ⌜W.1.1 !! i = Some (encode a)⌝.
+  Lemma sts_full_state_std W a b :
+    sts_full_world W -∗ sts_state_std a b -∗ ⌜W.1 !! a = Some b⌝.
   Proof.
     rewrite /sts_full_world /sts_full /sts_state_std.
-    (* iIntros "[% [H1 _]] H2". *)
-    destruct W as [[fs fr] Wloc]. 
-    iIntros "[[_ [_ [H1 _] ] ] _] H2". 
+    destruct W as [Wsta Wloc]. 
+    iIntros "[H1 _] H2". 
     iDestruct (own_valid_2 with "H1 H2") as %[HR Hv]%auth_both_valid;
       iPureIntro.
-    specialize (Hv i).
+    specialize (Hv a).
     revert HR; rewrite /= singleton_included;
       intros [z [Hz HR]].
     rewrite lookup_fmap in Hz Hv.
-    destruct (fs !! i) eqn:Heq; rewrite Heq /= in Hz Hv; last by inversion Hz.
+    destruct (Wsta !! a) eqn:Heq; rewrite Heq /= in Hz Hv; last by inversion Hz.
     apply leibniz_equiv in Hz; simplify_eq.
     apply Some_included_exclusive in HR; auto; last by typeclasses eauto.
     apply leibniz_equiv in HR; simplify_eq; eauto.
   Qed.
 
-  Lemma sts_full_state_loc W i b :
-    sts_full_world sts_std W -∗ sts_state_loc i b -∗ ⌜W.2.1 !! i = Some (encode b)⌝.
+  Lemma sts_full_state_loc W i d :
+    sts_full_world W -∗ sts_state_loc (A:=A) i d -∗ ⌜W.2.1 !! i = Some (encode d)⌝.
   Proof.
     rewrite /sts_full_world /sts_full /sts_state_loc.
-    (* iIntros "[% [H1 _]] H2". *)
     destruct W as [Wstd [fs fr] ]. 
     iIntros "[_ [H1 _]] H2". 
     iDestruct (own_valid_2 with "H1 H2") as %[HR Hv]%auth_both_valid;
@@ -421,38 +480,57 @@ Section STS.
     apply leibniz_equiv in HR; simplify_eq; eauto.
   Qed.
 
-  Lemma sts_dealloc_std W i a :
-    sts_full_world sts_std W ∗ sts_state_std i a ==∗ sts_full_world sts_std (delete i W.1.1,W.1.2,W.2). 
+  Lemma sts_dealloc_std W a b :
+    sts_full_world W ∗ sts_state_std a b ==∗ sts_full_world (delete a W.1,W.2). 
   Proof.
-    rewrite /sts_full_world /sts_full /sts_rel_std /sts_state_std.
-    destruct W as [[fs fr] Wloc]. 
-    iIntros "[ [[% [% [H1 H2] ] ] Hloc] Hstate] /=".
-    iCombine "H1" "Hstate" as "H1". 
+    rewrite /sts_full_world /sts_full /sts_state_std.
+    destruct W as [fs Wloc]. 
+    iIntros "[ [Hsta Hloc] Hstate] /=". 
+    iCombine "Hsta" "Hstate" as "H1". 
     iMod (own_update
-            (A := sts_stateUR)
+            (A := sts_std_stateUR A B)
             _ _
-            (● (Excl <$> (delete i fs)))
+            (● (Excl <$> (delete a fs)))
             with "H1") as "H1".
     { apply auth_update_dealloc.
       rewrite fmap_delete /=.
       apply: delete_singleton_local_update. }
-    iFrame. iModIntro. iPureIntro. split; auto.
-    etrans;[|eauto].
-    simpl. rewrite dom_delete_L.
-    by apply subseteq_difference_l. 
+    iFrame. iModIntro. done. 
   Qed. 
-    
-  Lemma sts_alloc_std W a :
-    sts_full_world sts_std W ==∗
-             ∃ i, sts_full_world sts_std (((<[i := encode a ]>W.1.1),(<[i := (convert_rel (Rpub : relation A),convert_rel (Rpriv : relation A)) ]>W.1.2)),W.2)
-                  ∗ ⌜i ∉ dom (gset positive) W.1.1⌝ ∗ ⌜i ∉ dom (gset positive) W.1.2⌝
-                  ∗ sts_state_std i a ∗ sts_rel_std sts_std i.
+
+  Lemma sts_alloc_std_i W a b :
+    ⌜a ∉ dom (gset A) W.1⌝ -∗
+    sts_full_world W ==∗
+    sts_full_world (<[a := b]>W.1,W.2) ∗ sts_state_std a b.
   Proof.
-    rewrite /sts_full_world /sts_full /sts_rel_std /sts_state_std.
+    rewrite /sts_full_world /sts_full /sts_state_std /=.
+    destruct W as [fsd Wloc]. rewrite /sts_full_std. 
+    iIntros (Hfresh1) "[H1 Hloc] /=".
+    iMod (own_update
+            (A := sts_std_stateUR A B)
+            _ _
+            (● (Excl <$> <[a :=b]> fsd)
+            ⋅ ◯ {[a := Excl b]})
+            with "H1") as "[H1 Hs]".
+    { apply auth_update_alloc.
+      rewrite fmap_insert /=.
+      apply: alloc_singleton_local_update; last done. 
+      apply (not_elem_of_dom (D := gset A)).
+      rewrite dom_fmap. auto. }
+    iFrame. done. 
+  Qed.
+
+  Lemma sts_alloc_loc W d Q P:
+    sts_full_world W ==∗
+             ∃ i, sts_full_world (W.1,((<[i := encode d ]>W.2.1),(<[i := (convert_rel Q,convert_rel P) ]>W.2.2)))
+                  ∗ ⌜i ∉ dom (gset positive) W.2.1⌝ ∗ ⌜i ∉ dom (gset positive) W.2.2⌝
+                  ∗ sts_state_loc (A:=A) i d ∗ sts_rel_loc (A:=A) i Q P.
+  Proof.
+    rewrite /sts_full_world /sts_full /sts_rel_loc /sts_state_loc.
     (* iIntros "[Hd [H1 H2]]". *)
     (* iDestruct "Hd" as %Hd. *)
-    destruct W as [[fs fr] Wloc]. 
-    iIntros "[[% [% [H1 H2] ] ] Hloc] /=".
+    destruct W as [Wstd [fs fr]]. 
+    iIntros "[Hstd [H1 H2]] /=".
     assert (fresh (dom (gset positive) fs ∪ dom (gset positive) fr) ∉
                     (dom (gset positive) fs ∪ dom (gset positive) fr)) as Hfresh.
     { apply is_fresh. }
@@ -461,120 +539,8 @@ Section STS.
             (A := sts_stateUR)
             _ _
             (● (Excl <$>
-                <[fresh (dom (gset positive) fs ∪ dom (gset positive) fr) := encode a]> fs)
-            ⋅ ◯ {[fresh (dom (gset positive) fs ∪ dom (gset positive) fr) := Excl (encode a)]})
-            with "H1") as "[H1 Hs]".
-    { apply auth_update_alloc.
-      rewrite fmap_insert /=.
-      apply: alloc_singleton_local_update; last done.
-      apply (not_elem_of_dom (D := gset positive)).
-      rewrite dom_fmap.
-      auto. }
-    iMod (own_update
-            (A := sts_relUR)
-            _ _
-            (● (to_agree <$>
-                <[fresh (dom (gset positive) fs ∪ dom (gset positive) fr) := (convert_rel Rpub,convert_rel Rpriv)]> fr)
-            ⋅ ◯ {[fresh (dom (gset positive) fs ∪ dom (gset positive) fr) := to_agree (convert_rel Rpub,convert_rel Rpriv)]})
-            with "H2") as "[H2 Hr]".
-    { apply auth_update_alloc.
-      rewrite fmap_insert /=.
-      apply: alloc_singleton_local_update; last done.
-      apply (not_elem_of_dom (D := gset positive)).
-      rewrite dom_fmap.
-      auto. }
-    iModIntro.
-    iExists _; iFrame.
-    repeat iSplit; auto.
-    - iPureIntro. do 2 rewrite dom_insert_L.
-      apply union_mono_l. auto. 
-    - iPureIntro. intros i [x Hx].
-      destruct (decide (fresh (dom (gset positive) fs ∪ dom (gset positive) fr) = i)).
-      + subst. rewrite lookup_insert. auto.
-      + rewrite lookup_insert_ne;auto. rewrite lookup_insert_ne in Hx; auto.
-        apply H3. eauto.       
-  Qed.
-
-  Lemma sts_alloc_std_i W i a :
-    ⌜i ∉ dom (gset positive) W.1.1⌝ -∗ (* ⌜i ∉ dom (gset positive) W.1.2⌝ -∗ *)
-    sts_full_world sts_std W ==∗
-                    sts_full_world sts_std (((<[i := encode a ]>W.1.1),(<[i := (convert_rel (Rpub : relation A),convert_rel (Rpriv: relation A)) ]>W.1.2)),W.2)
-                  ∗ sts_state_std i a.
-  Proof.
-    rewrite /sts_full_world /sts_full /sts_rel_std /sts_state_std /=.
-    (* iIntros "[Hd [H1 H2]]". *)
-    (* iDestruct "Hd" as %Hd. *)
-    destruct W as [[fs fr] Wloc]. rewrite /sts_full_std. 
-    iIntros (Hfresh1) "[[% [% [H1 H2] ] ] Hloc] /=".
-    iMod (own_update
-            (A := sts_stateUR)
-            _ _
-            (● (Excl <$>
-                <[i := encode a]> fs)
-            ⋅ ◯ {[i := Excl (encode a)]})
-            with "H1") as "[H1 Hs]".
-    { apply auth_update_alloc.
-      rewrite fmap_insert /=.
-      apply: alloc_singleton_local_update; last done.
-      apply (not_elem_of_dom (D := gset positive)).
-      rewrite dom_fmap.
-      auto. }
-    destruct (decide (i ∈ dom (gset positive) fr)). 
-    - (* i is already in the domain of fr. We know from sts_full_world that it must map to std_sts *)
-      apply elem_of_dom,H3 in e.
-      iFrame. iSplitR;[|iSplitR]. 
-      + iModIntro. iPureIntro. do 2 rewrite dom_insert_L.
-        apply union_mono_l. auto.
-      + iPureIntro. intros i0 [x Hx].
-        destruct (decide (i0 = i)).
-        * subst. rewrite lookup_insert. auto.
-        * rewrite lookup_insert_ne;auto. rewrite lookup_insert_ne in Hx; auto.
-          apply H3. eauto.
-      + rewrite (insert_id fr i (convert_rel Rpub, convert_rel Rpriv)); auto.
-    - iMod (own_update
-            (A := sts_relUR)
-            _ _
-            (● (to_agree <$>
-                <[i := (convert_rel Rpub,convert_rel Rpriv)]> fr)
-            ⋅ ◯ {[i := to_agree (convert_rel Rpub,convert_rel Rpriv)]})
-            with "H2") as "[H2 Hr]".
-      { apply auth_update_alloc.
-        rewrite fmap_insert /=.
-        apply: alloc_singleton_local_update; last done.
-        apply (not_elem_of_dom (D := gset positive)).
-        rewrite dom_fmap.
-        auto. }
-      iModIntro. iFrame. iSplit. 
-      + iPureIntro. do 2 rewrite dom_insert_L.
-        apply union_mono_l. auto.
-      + iPureIntro. intros i0 [x Hx].
-      destruct (decide (i0 = i)).
-        * subst. rewrite lookup_insert. auto.
-        * rewrite lookup_insert_ne;auto. rewrite lookup_insert_ne in Hx; auto.
-          apply H3. eauto.
-  Qed.
-
-  Lemma sts_alloc_loc W b Q P:
-    sts_full_world sts_std W ==∗
-             ∃ i, sts_full_world sts_std (W.1,((<[i := encode b ]>W.2.1),(<[i := (convert_rel Q,convert_rel P) ]>W.2.2)))
-                  ∗ ⌜i ∉ dom (gset positive) W.2.1⌝ ∗ ⌜i ∉ dom (gset positive) W.2.2⌝
-                  ∗ sts_state_loc i b ∗ sts_rel_loc i Q P.
-  Proof.
-    rewrite /sts_full_world /sts_full /sts_rel_loc /sts_state_loc.
-    (* iIntros "[Hd [H1 H2]]". *)
-    (* iDestruct "Hd" as %Hd. *)
-    destruct W as [Wstd [fs fr]]. 
-    iIntros "[Hstd [H1 H2]] /=".
-    assert (fresh (dom (gset positive) fs ∪ dom (gset positive) fr) ∉
-                    (dom (gset positive) fs ∪ dom (gset positive) fr)).
-    { apply is_fresh. }
-    apply not_elem_of_union in H2 as [Hfs Hfr]. 
-    iMod (own_update
-            (A := sts_stateUR)
-            _ _
-            (● (Excl <$>
-                <[fresh (dom (gset positive) fs ∪ dom (gset positive) fr) := encode b]> fs)
-            ⋅ ◯ {[fresh (dom (gset positive) fs ∪ dom (gset positive) fr) := Excl (encode b)]})
+                <[fresh (dom (gset positive) fs ∪ dom (gset positive) fr) := encode d]> fs)
+            ⋅ ◯ {[fresh (dom (gset positive) fs ∪ dom (gset positive) fr) := Excl (encode d)]})
             with "H1") as "[H1 Hs]".
     { apply auth_update_alloc.
       rewrite fmap_insert /=.
@@ -600,35 +566,32 @@ Section STS.
     repeat iSplit; auto. 
   Qed.
 
-  Lemma sts_update_std W i a a' :
-    sts_full_world sts_std W -∗ sts_state_std i a ==∗
-    sts_full_world sts_std (((<[i := encode a' ]>W.1.1),W.1.2),W.2) ∗ sts_state_std i a'.
+  Lemma sts_update_std W a b b' :
+    sts_full_world W -∗ sts_state_std a b ==∗
+    sts_full_world (<[a := b' ]>W.1,W.2) ∗ sts_state_std a b'.
   Proof.
     iIntros "Hsf Hi".
     iDestruct (sts_full_state_std with "Hsf Hi") as %Hfs.
-    rewrite /sts_full_world /sts_full /sts_rel_std /sts_state_std.
-    destruct W as [[fs fr] Wloc]. 
-    iDestruct "Hsf" as "[[% [% [H1 H2] ] ] Hloc] /=".
+    rewrite /sts_full_world /sts_full /sts_state_std.
+    destruct W as [fsd Wloc]. 
+    iDestruct "Hsf" as "[H1 Hloc] /=".
     iCombine "H1" "Hi" as "H1".
-    iMod (own_update (A := sts_stateUR)
+    iMod (own_update (A := sts_std_stateUR A B)
             _ _
-            (● (<[i := Excl (encode a')]> (Excl <$> fs))
-               ⋅ ◯ {[i := Excl (encode a')]})
+            (● (<[a := Excl b']> (Excl <$> fsd))
+               ⋅ ◯ {[a := Excl b']})
             with "H1") as "[H1 Hs]".
     { apply auth_update.
       apply: singleton_local_update; eauto.
       rewrite lookup_fmap Hfs //=.
       by apply exclusive_local_update. }
-    iFrame. rewrite fmap_insert (* dom_insert_L *) (* subseteq_union_1_L *);
-              first iModIntro; iFrame.  iSplit;auto.
-    iPureIntro.
-    rewrite dom_insert_L. rewrite subseteq_union_1_L; auto.
-    apply elem_of_subseteq_singleton. apply elem_of_gmap_dom. eauto. 
+    iFrame. rewrite -fmap_insert;
+              first iModIntro; iFrame.  
   Qed.
 
-  Lemma sts_update_loc W i b b' :
-    sts_full_world sts_std W -∗ sts_state_loc i b ==∗
-    sts_full_world sts_std (W.1,((<[i := encode b' ]>W.2.1),W.2.2)) ∗ sts_state_loc i b'.
+  Lemma sts_update_loc W i d d' :
+    sts_full_world W -∗ sts_state_loc (A:=A) i d ==∗
+    sts_full_world (W.1,((<[i := encode d' ]>W.2.1),W.2.2)) ∗ sts_state_loc (A:=A) i d'.
   Proof.
     iIntros "Hsf Hi".
     iDestruct (sts_full_state_loc with "Hsf Hi") as %Hfs.
@@ -638,8 +601,8 @@ Section STS.
     iCombine "H1" "Hi" as "H1".
     iMod (own_update (A := sts_stateUR)
             _ _
-            (● (<[i := Excl (encode b')]> (Excl <$> fs))
-               ⋅ ◯ {[i := Excl (encode b')]})
+            (● (<[i := Excl (encode d')]> (Excl <$> fs))
+               ⋅ ◯ {[i := Excl (encode d')]})
             with "H1") as "[H1 Hs]".
     { apply auth_update.
       apply: singleton_local_update; eauto.
